Makefile
@@ -27,7 +27,8 @@ all: $(VOFILES) LinearScan/Main.hs		\
 	@$(MAKE) LinearScan/Main.hs
 
 LinearScan/Main.hs: src/Main.vo
-	@mkdir LinearScan
+	@if [ ! -d LinearScan ]; then rm -f LinearScan; fi
+	@if [ ! -d LinearScan ]; then mkdir LinearScan; fi
 	@ls -1 *.hs | egrep -v '(Setup|LinearScan).hs' | \
 	    while read file; do mv $$file LinearScan; done
 	@perl -i fixcode.pl LinearScan/*.hs
